

25 Sep 2025

Thursday, September 25, 2025 2:00 PM

$E(X)$ is known as the First Moment

Moments: For each integer n , the n th moment of an r.v. X is: $E(X^n)$

The n th central moment is: $E(X - E(X))^n$

Variance is 2nd central moment: $VAR(X) = E(X - E(X))^2$

PROPERTIES OF VAR:

• $VAR(aX+b) = a^2 VAR(X)$

• $VAR(X) = E(X^2) - [E(X)]^2$

Ex. $X \sim \text{INV. GAMMA}(\alpha, \beta)$ $f(x) = \frac{1}{\Gamma(\alpha)\beta^\alpha} x^{-(\alpha+1)} e^{-\frac{1}{\beta}x}$

FROM LAST CLASS: $E(X) = \frac{1}{(\alpha-1)\beta}$

$E(X^2) = \int_0^\infty x^2 \frac{1}{\Gamma(\alpha)\beta^\alpha} x^{-(\alpha+1)} e^{-\frac{1}{\beta}x} dx = \frac{1}{\Gamma(\alpha)\beta^\alpha} \int_0^\infty x^{-(\alpha-1)} e^{-\frac{1}{\beta}x} dx = \frac{1}{\Gamma(\alpha)\beta^\alpha} \cdot \Gamma(\alpha-2) \beta^{\alpha-2}$
WITH $\Gamma(\alpha) = (\alpha-1)\Gamma(\alpha-1)$

$\therefore = \frac{1}{(\alpha-2)(\alpha-1)\beta^2}$

$\therefore VAR(X) = E(X^2) - E(X)^2 = \frac{1}{(\alpha-2)(\alpha-1)\beta^2} - \left(\frac{1}{(\alpha-1)\beta}\right)^2 = \frac{1}{(\alpha-2)(\alpha-1)^2\beta^2}$

Let's say instead of $E(X)$ we are interested in $E(Y)$ where $Y = g(X)$. Want to know: $E(g(X)) = g(E(X))$

This holds under very restrictive conditions, and often those are not met. However, we can usually compare

Jensen's inequality: a function $g(x)$ is convex if $g(\lambda x + (1-\lambda)y) \leq \lambda g(x) + (1-\lambda)g(y)$
 $\lambda \in [0,1], x,y \in \mathbb{R}$

IF $\lambda = \frac{1}{2}$: $g\left(\frac{x+y}{2}\right) \leq \frac{1}{2}(g(x) + g(y))$
 $g(x)$ IS CONCAVE IF $-g(x)$ IS CONVEX

HOW DETERMINE IF CONCAVE

• DRAW IT

• SECOND DERIVATIVE: IF $g''(x) > 0$, CONVEX

THEOREM: 4.7.7

IF $g(x)$ IS CONVEX, $E(g(x)) \geq g(E(x))$

IF $g(x)$ IS CONCAVE, $E(g(x)) \leq g(E(x))$

Ex. $g(x) = x^2$: CONVEX $\therefore E(x^2) \geq E(x)^2$

$g(x) = e^x$: CONVEX $\therefore E(e^x) \geq e^{E(x)}$

$g(x) = \ln(x)$: CONCAVE $\therefore E(\ln(x)) \leq \ln(E(x))$

Ex. DIFF MEANS OF POS. NUMS.

$$a_A = \frac{1}{n}(a_1 + a_2 + \dots + a_n)$$

$$a_G = \left(a_1 + a_2 + \dots + a_n \right)^{\frac{1}{n}}$$

$$a_H = \frac{1}{\frac{1}{n}(a_1 + a_2 + \dots + a_n)} \quad \text{PROVE: } a_H \leq a_G \leq a_A$$

X IS R.V. WITH SUPPORT (a_1, a_2, \dots, a_n) ; $P(X = a_i) = \frac{1}{n}$

$$E(X) = \sum_{i=1}^n a_i P(X=a_i) = \frac{1}{n} \sum_{i=1}^n a_i$$

$$\log(a_G) = \frac{1}{n} \sum_{i=1}^n \log(a_i) = E(\log(X)) \leq \log(E(X)) = \log\left(\frac{1}{n} \sum_{i=1}^n a_i\right) = \log(a_A) \Rightarrow a_G \leq a_A$$

$$\log\left(\frac{1}{a_H}\right) = \log\left(\frac{1}{\frac{1}{n} \sum_{i=1}^n \frac{1}{a_i}}\right) = \log(E(\frac{1}{X})) \geq E(\log(\frac{1}{X})) = -E(\log(X)) = -\log(a_G) = \log\left(\frac{1}{a_G}\right)$$

$$\therefore \frac{1}{a_H} \geq \frac{1}{a_G} \therefore a_H \leq a_G$$

Moment Generating Function (MGF)

X IS R.V. WITH CDF $F_X(x)$, THE MGF OF X IS:

$$M_X(t) = E(e^{tx}) = \begin{cases} \int_{-\infty}^{\infty} e^{tx} f_X(x) dx & X \text{ IS CONT.} \\ \sum_{x \in X} e^{tx} f_X(x) & \text{DISCRETE} \end{cases}$$

This holds if the expectation exists for t in the neighborhood of 0. That is, there exists an $h > 0$ such that $E(e^{tx})$ exists for all $-h < t < h$

$$\text{THM: IF } X \text{ HAS MGF: } M_X(t), \text{ THEN } E(X^n) = M_X^{(n)}(0) = \frac{d^n}{dt^n} M_X(t) \Big|_{t=0}$$

Proof: (start with assumption that we can bring the derivative inside the integral, see section 2.4 in CB)

$$\begin{aligned} \frac{d^n}{dt^n} M_X(t) \Big|_{t=0} &= \left[\frac{d^n}{dt^n} \int e^{tx} f_X(x) dx \right] \Big|_{t=0} = \left[\int \underbrace{\frac{d^n}{dt^n} e^{tx}}_{x^n e^{tx}} f_X(x) dx \right] \Big|_{t=0} \\ &= \left[\int x^n e^{tx} f_X(x) dx \right] \Big|_{t=0} = E(X^n e^{tx}) \Big|_{t=0} = E(X^n) \end{aligned}$$

Ex. X IS EXP. R.V. w/ $f(x) = \frac{1}{\theta} e^{-x/\theta}$ $x > 0$
 $\theta > 0$

$$M_X(t) = E(e^{tx}) = \int_0^{\infty} e^{tx} \frac{1}{\theta} e^{-x/\theta} dx = \frac{1}{\theta} \int_0^{\infty} e^{-x(\frac{1}{\theta} - t)} dx = \frac{1}{\theta} \int_0^{\infty} e^{-x(\frac{1-t\theta}{\theta})} dx$$

$$= \frac{1}{\theta} \frac{1}{\frac{1-t\theta}{\theta}} = \frac{1}{1-t\theta}$$

$$E(X) = M_X'(0) \Rightarrow \frac{d}{dt} \frac{1}{1-t\theta} = \frac{d}{dt} (1-t\theta)^{-1} = \frac{\theta}{(1-t\theta)^2} \therefore E(X) = M_X'(0) = \frac{\theta}{(1-0)^2} = \theta$$

$$E(X^2) = M_X''(0) \quad \frac{d^2}{dt^2} \frac{1}{1-t\theta} = \frac{2\theta^2}{(1-t\theta)^3} \therefore E(X^2) = 2\theta^2$$

$$\therefore \text{VAR}(X) = E(X^2) - E(X)^2 = 2\theta^2 - \theta^2 = \theta^2$$